Adapt safechecker to a new wf_env record, storing both an efficient declaration lookup table and the graph

safechecker/theories/PCUICSafeChecker.v
@@ -237,35 +237,6 @@ Section CheckEnv.
     easy.
   Defined.
 
-  (* We pack up all the information required on the global environment and graph in a 
-    single record. *)
-
-  Record wf_env {cf:checker_flags} := { 
-    wf_env_env :> global_env;
-    wf_env_wf :> ∥ wf wf_env_env ∥;
-    wf_env_graph :> universes_graph;
-    wf_env_graph_wf : is_graph_of_uctx wf_env_graph (global_uctx wf_env_env)
-  }.
-
-  Record wf_env_ext {cf:checker_flags} := { 
-      wf_env_ext_env :> global_env_ext;
-      wf_env_ext_wf :> ∥ wf_ext wf_env_ext_env ∥;
-      wf_env_ext_graph :> universes_graph;
-      wf_env_ext_graph_wf : is_graph_of_uctx wf_env_ext_graph (global_ext_uctx wf_env_ext_env)
-  }.
-
-  Definition wf_env_sq_wf (Σ : wf_env) : ∥ wf Σ ∥.
-  Proof.
-    destruct (wf_env_wf Σ).
-    sq. apply X.
-  Qed.
-  
-  Definition wf_env_ext_sq_wf (Σ : wf_env_ext) : ∥ wf Σ ∥.
-  Proof.
-    destruct (wf_env_ext_wf Σ).
-    sq. apply X.
-  Qed.
-
   Section UniverseChecks.
   Obligation Tactic := idtac.
  
