safechecker/theories/PCUICEnvMap.v
@@ -1,0 +1,219 @@
+
+(* Distributed under the terms of the MIT license. *)
+From Coq Require Import ssreflect PArith.BinPos PArith.
+From MetaCoq.Template Require Import config utils uGraph Reflect String2pos CanonicalTries.
+From MetaCoq.PCUIC Require Import PCUICAst PCUICAstUtils
+     PCUICReflect PCUICTyping PCUICGlobalEnv PCUICTyping.
+From Equations Require Import Equations.
+
+(* Implementation of environment lookup using efficient canonical tries by Appel & Leroy *)
+
+Implicit Types (cf:checker_flags).
+
+Module EnvMap.
+  Definition t := PTree.tree global_decl.
+
+  Lemma bool_cons_pos_inj a a' p p' : bool_cons_pos a p = bool_cons_pos a' p' -> a = a' /\ p = p'.
+  Proof.
+    destruct a, a'; cbn; try discriminate; intros [=] => //.
+  Qed.
+
+  Lemma ascii_cons_pos_inj a a' p p' : ascii_cons_pos a p = ascii_cons_pos a' p' -> a = a' /\ p = p'.
+  Proof.
+    unfold ascii_cons_pos.
+    destruct a, a'.
+    repeat move/bool_cons_pos_inj => [] ?; subst; auto.
+  Qed.
+  
+  Lemma pos_of_string_inj s s' : pos_of_string s = pos_of_string s' -> s = s'.
+  Proof.
+    induction s in s' |- *; destruct s' => /= //.
+    destruct a. cbn. destruct b; cbn; discriminate.
+    destruct a. cbn. destruct b; cbn; discriminate.
+    move/ascii_cons_pos_inj. intuition f_equal; auto.
+  Qed.
+
+  Fixpoint pos_of_string_cont (s: string) (p : positive) : positive :=
+    match s with
+    | EmptyString => Pos.succ p
+    | String c s => ascii_cons_pos c (pos_of_string_cont s p)
+    end.
+(*   
+  Lemma ascii_cons_pos_plus a p : 
+    ascii_cons_pos a (Pos.succ p) = (Pos.iter xO (ascii_cons_pos a 1) p)%positive.
+  Proof.
+    
+   *)
+  (* Lemma ascii_cons_pos_plus a p p' : 
+    ascii_cons_pos a (p + p')%positive = (ascii_cons_pos a p + p')%positive.
+  Proof.
+    induction p using Pos.peano_ind.
+    -  simpl. destruct p'; cbn.
+      rewrite Pos.xI_succ_xO.
+      cbn. *)
+
+  
+  (* Lemma ascii_cons_pos_shiftl a p n p' : 
+    ascii_cons_pos a (Pos.shiftl p (N.pos n) + p') = ((Pos.iter xO (ascii_cons_pos a p) n) + p')%positive.
+  Proof.
+    induction n using Pos.peano_ind.
+    - cbn. destruct p'.
+      2:{ rewrite !Pos.add_xO.
+
+      all:admit.
+    - cbn. rewrite !Pos.iter_succ.
+      destruct p'.
+      * cbn ,
+      rewrite Pos.add_xO.
+      cbn.
+
+ *)
+
+  Lemma pos_of_string_cont_spec s p : pos_of_string_cont s p = 
+    (Pos.shiftl (pos_of_string s) (N.of_nat (String.length s)) + p)%positive.
+  Proof.
+    induction s.
+    - cbn. now destruct p; cbn.
+    - cbn. rewrite IHs.
+  Admitted.
+
+
+  Lemma pos_of_string_cont_inj s s' p : pos_of_string_cont s p = pos_of_string_cont s' p -> s = s'.
+  Proof.
+    induction s; destruct s' => /= //.
+  Admitted.
+  
+  Fixpoint pos_of_dirpath_cont (d : dirpath) (cont : positive) : positive := 
+    match d with
+    | hd :: tl => pos_of_string_cont hd (pos_of_dirpath_cont tl cont)
+    | [] => cont
+    end.
+
+  Fixpoint pos_of_nat_cont (n : nat) (cont : positive) : positive :=
+    match n with
+    | 0 => cont
+    | S x => Pos.succ (pos_of_nat_cont x cont)
+    end.
+
+  Fixpoint pos_of_modpath_cont (m : modpath) (p : positive) : positive :=
+    match m with
+    | MPfile d => pos_of_dirpath_cont d p
+    | MPbound d i k => pos_of_dirpath_cont d (pos_of_string_cont i (pos_of_nat_cont k p))
+    | MPdot m i => pos_of_modpath_cont m (pos_of_string_cont i p)
+    end.
+
+  Definition pos_of_kername (k : kername) : positive :=
+    pos_of_modpath_cont k.1 (pos_of_string k.2).
+  
+  Lemma pos_of_kername_inj k k' : pos_of_kername k = pos_of_kername k' -> k = k'.
+  Proof.
+    induction k; destruct k'.
+    unfold pos_of_kername. cbn.
+    induction a; destruct m => /= //.
+
+    cbn.
+  Admitted.
+
+  Definition empty : t := PTree.empty _.
+
+  Definition lookup (k : kername) (env : t) : option global_decl :=
+    PTree.get (pos_of_kername k) env.
+
+  Definition add (k : kername) (g : global_decl) (env : t) : t :=
+    PTree.set (pos_of_kername k) g env.
+
+  Definition of_global_env (g : global_env) : t :=
+    List.fold_left (fun genv decl => add decl.1 decl.2 genv) g empty.
+    
+  Definition repr (g : global_env) (e : t) := e = of_global_env g.
+  Arguments PTree.set : simpl never.
+
+  Lemma of_global_env_comm {cf:checker_flags} g d d' : 
+    fresh_global d.1 (d' :: g) -> fresh_global d'.1 g ->
+    of_global_env (d :: d' :: g) = of_global_env (d' :: d :: g).
+  Proof.
+    intros hwf hwf'.
+    cbn. f_equal. apply PTree.extensionality.
+    intros i.
+    unfold add.
+    destruct (Pos.eq_dec i (pos_of_kername d'.1)).
+    - subst. rewrite PTree.gss PTree.gso.
+      intros eq. apply pos_of_kername_inj in eq. depelim hwf. cbn in H; congruence.
+      now rewrite PTree.gss.
+    - rewrite PTree.gso //.
+      destruct (Pos.eq_dec i (pos_of_kername d.1)); [subst i|].
+      + rewrite !PTree.gss //.
+      + rewrite !PTree.gso //.
+  Qed.
+
+  Lemma add_comm g d d' : 
+    d.1 <> d'.1 -> add d.1 d.2 (add d'.1 d'.2 g) = add d'.1 d'.2 (add d.1 d.2 g).
+  Proof.
+    intros hwf.
+    cbn. unfold add. apply PTree.extensionality=> i.
+    destruct (Pos.eq_dec i (pos_of_kername d'.1)).
+    - subst. rewrite PTree.gss PTree.gso.
+      intros eq. apply pos_of_kername_inj in eq. congruence.
+      now rewrite PTree.gss.
+    - destruct (Pos.eq_dec i (pos_of_kername d.1)); [subst i|].
+      + rewrite !PTree.gss // PTree.gso // !PTree.gss //.
+      + rewrite !PTree.gso //.
+  Qed.
+
+  Inductive fresh_globals : global_env -> Prop :=
+    | fresh_globals_empty : fresh_globals []
+    | fresh_globals_cons kn d g : 
+      fresh_globals g -> fresh_global kn g ->
+      fresh_globals ((kn, d) :: g). 
+  Derive Signature for fresh_globals.
+
+  Lemma fold_left_cons d g acc :
+    fold_left (fun (genv : t) (decl : kername × global_decl) => add decl.1 decl.2 genv) (d :: g) acc = 
+    fold_left (fun (genv : t) (decl : kername × global_decl) => add decl.1 decl.2 genv) g (add d.1 d.2 acc).
+  Proof. reflexivity. Qed.
+  
+  Lemma of_global_env_cons {cf:checker_flags} d g : fresh_globals (d :: g) ->
+    of_global_env (d :: g) = add d.1 d.2 (of_global_env g).
+  Proof.
+    unfold of_global_env. generalize empty.
+    induction g.
+    - cbn; auto.
+    - unfold fresh_global.
+      intros acc hf. depelim hf.
+      rewrite fold_left_cons. rewrite -IHg. constructor. now depelim hf. now depelim H.
+      cbn. f_equal. rewrite (add_comm _ a (kn, d0)) //. cbn. now depelim H.
+  Qed.
+
+  Lemma wf_fresh_globals {cf} Σ : wf Σ -> fresh_globals Σ.
+  Proof. induction 1; constructor; auto. Qed.
+
+  Lemma lookup_add k v g : lookup k (add k v g) = Some v.
+  Proof. rewrite /lookup /add. rewrite PTree.gss //. Qed.
+
+  Lemma lookup_add_other k k' v g : k <> k' -> lookup k (add k' v g) = lookup k g.
+  Proof. move=> eqk. rewrite /lookup /add. rewrite PTree.gso //.
+    move/pos_of_kername_inj. congruence. 
+  Qed.
+
+  Lemma lookup_env_head d g : lookup_env (d :: g) d.1 = Some d.2.
+  Proof.
+    now rewrite /lookup_env eq_kername_refl.
+  Qed.
+
+  Lemma lookup_spec {cf : checker_flags} (g : global_env) (e : t) : wf g ->
+    repr g e ->
+    forall k, lookup k e = lookup_env g k.
+  Proof.
+    intros wf -> k.
+    induction g in k, wf |- *; auto.
+    change (eq_kername k a.1) with (eqb k a.1).
+    destruct (eqb_spec k a.1).
+    - subst. rewrite of_global_env_cons; [now apply wf_fresh_globals|].
+      now rewrite lookup_add lookup_env_head.
+    - rewrite of_global_env_cons. now apply wf_fresh_globals.
+      rewrite lookup_add_other //. destruct a; rewrite lookup_env_cons_fresh //.
+      * cbn in n. congruence.
+      * apply IHg. now depelim wf.
+  Qed.
+
+End EnvMap.
