template-coq/theories/utils/canonicaltries/String2pos.v
@@ -1,0 +1,38 @@
+(** Convert strings to positive numbers.
+    The encoding used is the trivial one (8 bits per character). *)
+
+    From Coq Require Import String Ascii ZArith Extraction.
+
+    Definition bool_cons_pos (b: bool) (n: positive) : positive :=
+      if b then xI n else xO n.
+    
+    Definition ascii_cons_pos (c: ascii) (n: positive) : positive :=
+      match c with
+      | Ascii b0 b1 b2 b3 b4 b5 b6 b7 =>
+          bool_cons_pos b0 (
+          bool_cons_pos b1 (
+          bool_cons_pos b2 (
+          bool_cons_pos b3 (
+          bool_cons_pos b4 (
+          bool_cons_pos b5 (
+          bool_cons_pos b6 (
+          bool_cons_pos b7 n)))))))
+      end.
+    
+    Extract Constant ascii_cons_pos =>
+      "(fun c n ->
+          let c = Char.code c in
+          let n1 = if c land 1 = 0 then XO n else XI n in
+          let n2 = if c land 2 = 0 then XO n1 else XI n1 in
+          let n3 = if c land 4 = 0 then XO n2 else XI n2 in
+          let n4 = if c land 8 = 0 then XO n3 else XI n3 in
+          let n5 = if c land 16 = 0 then XO n4 else XI n4 in
+          let n6 = if c land 32 = 0 then XO n5 else XI n5 in
+          let n7 = if c land 64 = 0 then XO n6 else XI n6 in
+          if c land 128 = 0 then XO n7 else XI n7)".
+    
+    Fixpoint pos_of_string (s: string) : positive :=
+      match s with
+      | EmptyString => xH
+      | String c s => ascii_cons_pos c (pos_of_string s)
+      end.
